zoo_saturn/spsc_bqueue: Rewrite.

theories/zoo_saturn/spsc_bqueue.v
@@ -8,7 +8,7 @@ From zoo.common Require Import
   relations
   list.
 From zoo.iris.base_logic Require Import
-  lib.excl
+  lib.twins
   lib.auth_twins
   lib.auth_nat_max
   lib.mono_list.
@@ -33,18 +33,26 @@ Implicit Types l : location.
 Implicit Types v w t : val.
 Implicit Types vs ws hist : list val.
 
+Inductive stability :=
+  | Stable
+  | Unstable.
+Implicit Types stable : stability.
+
+#[local] Instance stability_inhabited : Inhabited stability :=
+  populate Stable.
+
 Class SpscBqueueG Σ `{zoo_G : !ZooG Σ} := {
   #[local] spsc_bqueue_G_model_G :: AuthTwinsG Σ (leibnizO (list val)) suffix ;
   #[local] spsc_bqueue_G_history_G :: MonoListG Σ val ;
-  #[local] spsc_bqueue_G_ctl_G :: AuthNatMaxG Σ ;
-  #[local] spsc_bqueue_G_region_G :: ExclG Σ unitO ;
+  #[local] spsc_bqueue_G_stability_G :: TwinsG Σ (leibnizO stability) ;
+  #[local] spsc_bqueue_G_mono_nat_G :: AuthNatMaxG Σ ;
 }.
 
 Definition spsc_bqueue_Σ := #[
   auth_twins_Σ (leibnizO (list val)) suffix ;
   mono_list_Σ val ;
-  auth_nat_max_Σ ;
-  excl_Σ unitO
+  twins_Σ (leibnizO stability) ;
+  auth_nat_max_Σ
 ].
 Lemma subG_spsc_bqueue_Σ Σ `{zoo_G : !ZooG Σ} :
   subG spsc_bqueue_Σ Σ →
@@ -61,10 +69,10 @@ Section spsc_bqueue_G.
     metadata_data : val ;
     metadata_model : auth_twins_name ;
     metadata_history : gname ;
-    metadata_producer_ctl : gname ;
-    metadata_producer_region : gname ;
-    metadata_consumer_ctl : gname ;
-    metadata_consumer_region : gname ;
+    metadata_producer : gname ;
+    metadata_back : gname ;
+    metadata_consumer : gname ;
+    metadata_front : gname ;
   }.
   Implicit Types γ : metadata.
 
@@ -92,67 +100,83 @@ Section spsc_bqueue_G.
   #[local] Definition history_at γ :=
     mono_list_at γ.(metadata_history).
 
-  #[local] Definition producer_ctl₁' γ_producer_ctl γ_model back ws : iProp Σ :=
-    auth_nat_max_auth γ_producer_ctl (DfracOwn (1/2)) back ∗
+  #[local] Definition producer₁' γ_producer γ_back γ_model stable back ws : iProp Σ :=
+    twins_twin1 γ_producer (DfracOwn 1) stable ∗
+    auth_nat_max_auth γ_back (DfracOwn (1/2)) back ∗
     auth_twins_auth _ (auth_twins_G := spsc_bqueue_G_model_G) γ_model ws.
-  #[local] Definition producer_ctl₁ γ :=
-    producer_ctl₁' γ.(metadata_producer_ctl) γ.(metadata_model).
-  #[local] Instance : CustomIpatFormat "producer_ctl₁" :=
+  #[local] Definition producer₁ γ :=
+    producer₁' γ.(metadata_producer) γ.(metadata_back) γ.(metadata_model).
+  #[local] Instance : CustomIpatFormat "producer₁" :=
     "(
-      Hproducer_ctl₁ &
+      Hproducer₁ &
+      Hback_auth₁ &
       Hmodel_auth
     )".
-  #[local] Definition producer_ctl₂' γ_producer_ctl :=
-    auth_nat_max_auth γ_producer_ctl (DfracOwn (1/2)).
-  #[local] Definition producer_ctl₂ γ :=
-    producer_ctl₂' γ.(metadata_producer_ctl).
+  #[local] Definition producer₂' γ_producer γ_back stable back : iProp Σ :=
+    twins_twin2 γ_producer stable ∗
+    auth_nat_max_auth γ_back (DfracOwn (1/2)) back.
+  #[local] Definition producer₂ γ :=
+    producer₂' γ.(metadata_producer) γ.(metadata_back).
+  #[local] Instance : CustomIpatFormat "producer₂" :=
+    "(
+      Hproducer₂ &
+      Hback_auth₂
+    )".
   #[local] Definition back_lb γ :=
-    auth_nat_max_lb γ.(metadata_producer_ctl).
+    auth_nat_max_lb γ.(metadata_back).
 
-  #[local] Definition producer_region' γ_producer_region :=
-    excl γ_producer_region ().
-  #[local] Definition producer_region γ :=
-    producer_region' γ.(metadata_producer_region).
-
-  #[local] Definition consumer_ctl₁' γ_consumer_ctl :=
-    auth_nat_max_auth γ_consumer_ctl (DfracOwn (1/2)).
-  #[local] Definition consumer_ctl₁ γ :=
-    consumer_ctl₁' γ.(metadata_consumer_ctl).
-  #[local] Definition consumer_ctl₂' γ_consumer_ctl :=
-    auth_nat_max_auth γ_consumer_ctl (DfracOwn (1/2)).
-  #[local] Definition consumer_ctl₂ γ :=
-    consumer_ctl₂' γ.(metadata_consumer_ctl).
+  #[local] Definition consumer₁' γ_consumer γ_front stable front : iProp Σ :=
+    twins_twin1 γ_consumer (DfracOwn 1) stable ∗
+    auth_nat_max_auth γ_front (DfracOwn (1/2)) front.
+  #[local] Definition consumer₁ γ :=
+    consumer₁' γ.(metadata_consumer) γ.(metadata_front).
+  #[local] Instance : CustomIpatFormat "consumer₁" :=
+    "(
+      Hconsumer₁ &
+      Hfront_auth₁
+    )".
+  #[local] Definition consumer₂' γ_consumer γ_front stable front : iProp Σ :=
+    twins_twin2 γ_consumer stable ∗
+    auth_nat_max_auth γ_front (DfracOwn (1/2)) front.
+  #[local] Definition consumer₂ γ :=
+    consumer₂' γ.(metadata_consumer) γ.(metadata_front).
+  #[local] Instance : CustomIpatFormat "consumer₂" :=
+    "(
+      Hconsumer₂ &
+      Hfront_auth₂
+    )".
   #[local] Definition front_lb γ :=
-    auth_nat_max_lb γ.(metadata_consumer_ctl).
-
-  #[local] Definition consumer_region' γ_consumer_region :=
-    excl γ_consumer_region ().
-  #[local] Definition consumer_region γ :=
-    consumer_region' γ.(metadata_consumer_region).
+    auth_nat_max_lb γ.(metadata_front).
 
   #[local] Definition inv_inner l γ : iProp Σ :=
-    ∃ front back vs hist,
+    ∃ cstable front pstable back vs hist,
     ⌜back = (front + length vs)%nat⌝ ∗
     ⌜back ≤ front + γ.(metadata_capacity)⌝ ∗
     ⌜length hist = back⌝ ∗
     ⌜vs = drop front hist⌝ ∗
     l.[front] ↦ #front ∗
-    consumer_ctl₂ γ front ∗
+    consumer₂ γ cstable front ∗
     l.[back] ↦ #back ∗
-    producer_ctl₂ γ back ∗
+    producer₂ γ pstable back ∗
     model₂ γ vs ∗
     history_auth γ hist ∗
-    ( array_cslice γ.(metadata_data) γ.(metadata_capacity) front (DfracOwn 1) ((λ v, ‘Some( v )%V) <$> take 1 vs)
-    ∨ consumer_region γ
+    ( if cstable then
+        array_cslice γ.(metadata_data) γ.(metadata_capacity) front (DfracOwn 1) ((λ v, ‘Some( v )%V) <$> take 1 vs)
+      else
+        True
     ) ∗
     array_cslice γ.(metadata_data) γ.(metadata_capacity) (S front) (DfracOwn 1) ((λ v, ‘Some( v )%V) <$> drop 1 vs) ∗
-    ( array_cslice γ.(metadata_data) γ.(metadata_capacity) back (DfracOwn 1) (if decide (back = front + γ.(metadata_capacity)) then [] else [§None%V])
-    ∨ producer_region γ
+    ( if pstable then
+        array_cslice γ.(metadata_data) γ.(metadata_capacity) back (DfracOwn 1) (if decide (back = front + γ.(metadata_capacity)) then [] else [§None%V])
+      else
+        True
     ) ∗
     array_cslice γ.(metadata_data) γ.(metadata_capacity) (S back) (DfracOwn 1) (replicate (γ.(metadata_capacity) - (back - front) - 1) §None%V).
   #[local] Instance : CustomIpatFormat "inv_inner" :=
     "(
+      %cstable{} &
       %front{} &
+      %pstable{} &
       %back{} &
       %vs{} &
       %hist{} &
@@ -161,9 +185,9 @@ Section spsc_bqueue_G.
       >%Hhist{}_len &
       >%Hvs{} &
       >Hl_front &
-      >Hconsumer_ctl₂ &
+      >Hconsumer₂ &
       >Hl_back &
-      >Hproducer_ctl₂ &
+      >Hproducer₂ &
       >Hmodel₂ &
       >Hhistory_auth &
       >Hfront &
@@ -210,8 +234,7 @@ Section spsc_bqueue_G.
     ⌜t = #l⌝ ∗
     meta l nroot γ ∗
     l.[front_cache] ↦ #front_cache ∗
-    producer_ctl₁ γ back ws ∗
-    producer_region γ ∗
+    producer₁ γ Stable back ws ∗
     front_lb γ front_cache.
   #[local] Instance : CustomIpatFormat "producer" :=
     "(
@@ -222,8 +245,7 @@ Section spsc_bqueue_G.
       {{}->=%Heq} &
       #Hmeta{{}=_} &
       Hl_front_cache &
-      Hproducer_ctl₁ &
-      Hproducer_region &
+      Hproducer₁ &
       #Hfront_lb
     )".
 
@@ -232,8 +254,7 @@ Section spsc_bqueue_G.
     ⌜t = #l⌝ ∗
     meta l nroot γ ∗
     l.[back_cache] ↦ #back_cache ∗
-    consumer_ctl₁ γ front ∗
-    consumer_region γ ∗
+    consumer₁ γ Stable front ∗
     back_lb γ back_cache.
   #[local] Instance : CustomIpatFormat "consumer" :=
     "(
@@ -244,8 +265,7 @@ Section spsc_bqueue_G.
       %Heq &
       #Hmeta_ &
       Hl_back_cache &
-      Hconsumer_ctl₁ &
-      Hconsumer_region &
+      Hconsumer₁ &
       #Hback_lb
     )".
 
@@ -259,8 +279,18 @@ Section spsc_bqueue_G.
   Proof.
     apply _.
   Qed.
+  #[local] Instance producer₂_timeless γ stable back :
+    Timeless (producer₂ γ stable back).
+  Proof.
+    apply _.
+  Qed.
   #[global] Instance spsc_bqueue_producer_timeless t ws :
     Timeless (spsc_bqueue_producer t ws).
+  Proof.
+    apply _.
+  Qed.
+  #[local] Instance consumer₂_timeless γ stable front :
+    Timeless (consumer₂ γ stable front).
   Proof.
     apply _.
   Qed.
@@ -270,24 +300,25 @@ Section spsc_bqueue_G.
     apply _.
   Qed.
 
-  #[local] Lemma model_producer_ctl_alloc :
+  #[local] Lemma model_producer_alloc :
     ⊢ |==>
-      ∃ γ_model γ_producer_ctl,
+      ∃ γ_model γ_producer γ_back,
       model₁' γ_model [] ∗
       model₂' γ_model [] ∗
-      producer_ctl₁' γ_producer_ctl γ_model 0 [] ∗
-      producer_ctl₂' γ_producer_ctl 0.
+      producer₁' γ_producer γ_back γ_model Stable 0 [] ∗
+      producer₂' γ_producer γ_back Stable 0.
   Proof.
     iMod (auth_twins_alloc (auth_twins_G := spsc_bqueue_G_model_G) _ []) as "(%γ_model & Hmodel_auth & Hmodel₁ & Hmodel₂)".
-    iMod auth_nat_max_alloc as "(%γ_producer_ctl & Hproducer_ctl₁ & Hproducer_ctl₂)".
+    iMod twins_alloc' as "(%γ_producer & Hproducer₁ & Hproducer₂)".
+    iMod auth_nat_max_alloc as "(%γ_back & Hback_auth₁ & Hback_auth₂)".
     iSteps.
   Qed.
-  #[local] Lemma model_valid γ back ws vs :
-    producer_ctl₁ γ back ws -∗
+  #[local] Lemma model_valid γ stable back ws vs :
+    producer₁ γ stable back ws -∗
     model₁ γ vs -∗
     ⌜vs `suffix_of` ws⌝.
   Proof.
-    iIntros "(:producer_ctl₁) Hmodel₁".
+    iIntros "(:producer₁) Hmodel₁".
     iDestruct (auth_twins_valid_1 with "Hmodel_auth Hmodel₁") as %H.
     rewrite preorder_rtc in H. iSteps.
   Qed.
@@ -300,15 +331,15 @@ Section spsc_bqueue_G.
     iDestruct (auth_twins_agree_L with "Hmodel₁ Hmodel₂") as %->.
     iSteps.
   Qed.
-  #[local] Lemma model_push {γ back ws vs1 vs2} v :
-    producer_ctl₁ γ back ws -∗
+  #[local] Lemma model_push {γ stable back ws vs1 vs2} v :
+    producer₁ γ stable back ws -∗
     model₁ γ vs1 -∗
     model₂ γ vs2 ==∗
-      producer_ctl₁ γ back (vs1 ++ [v]) ∗
+      producer₁ γ stable back (vs1 ++ [v]) ∗
       model₁ γ (vs1 ++ [v]) ∗
       model₂ γ (vs1 ++ [v]).
   Proof.
-    iIntros "(:producer_ctl₁) Hmodel₁ Hmodel₂".
+    iIntros "(:producer₁) Hmodel₁ Hmodel₂".
     iMod (auth_twins_update_auth with "Hmodel_auth Hmodel₁ Hmodel₂") as "(Hmodel_auth & Hmodel₁ & Hmodel₂)".
     iSteps.
   Qed.
@@ -352,114 +383,120 @@ Section spsc_bqueue_G.
     apply mono_list_update_snoc.
   Qed.
 
-  #[local] Lemma producer_ctl_agree γ back1 ws back2 :
-    producer_ctl₁ γ back1 ws -∗
-    producer_ctl₂ γ back2 -∗
-    ⌜back1 = back2⌝.
+  #[local] Lemma producer_agree γ stable1 back1 ws stable2 back2 :
+    producer₁ γ stable1 back1 ws -∗
+    producer₂ γ stable2 back2 -∗
+      ⌜stable1 = stable2⌝ ∗
+      ⌜back1 = back2⌝.
   Proof.
-    iIntros "(:producer_ctl₁) Hproducer_ctl₂".
-    iApply (auth_nat_max_auth_agree with "Hproducer_ctl₁ Hproducer_ctl₂").
+    iIntros "(:producer₁) (:producer₂)".
+    iDestruct (twins_agree_L with "Hproducer₁ Hproducer₂") as %<-.
+    iDestruct (auth_nat_max_auth_agree with "Hback_auth₁ Hback_auth₂") as %<-.
+    iSteps.
   Qed.
-  #[local] Lemma producer_ctl_update {γ back1 ws back2} back :
+  #[local] Lemma producer_update_stability {γ stable1 back1 ws stable2 back2} stable :
+    producer₁ γ stable1 back1 ws -∗
+    producer₂ γ stable2 back2 ==∗
+      producer₁ γ stable back1 ws ∗
+      producer₂ γ stable back2.
+  Proof.
+    iIntros "(:producer₁) (:producer₂)".
+    iMod (twins_update' with "Hproducer₁ Hproducer₂") as "(Hproducer₁ & Hproducer₂)".
+    iSteps.
+  Qed.
+  #[local] Lemma producer_update_back {γ stable1 back1 ws stable2 back2} back :
     back1 ≤ back →
-    producer_ctl₁ γ back1 ws -∗
-    producer_ctl₂ γ back2 ==∗
-      producer_ctl₁ γ back ws ∗
-      producer_ctl₂ γ back.
+    producer₁ γ stable1 back1 ws -∗
+    producer₂ γ stable2 back2 ==∗
+      producer₁ γ stable1 back ws ∗
+      producer₂ γ stable2 back.
   Proof.
-    iIntros "% (:producer_ctl₁) Hproducer_ctl₂".
-    iDestruct (auth_nat_max_auth_agree with "Hproducer_ctl₁ Hproducer_ctl₂") as %->.
-    iCombine "Hproducer_ctl₁ Hproducer_ctl₂" as "Hproducer_ctl".
-    iMod (auth_nat_max_update with "Hproducer_ctl") as "($ & $)"; done.
+    iIntros "% (:producer₁) (:producer₂)".
+    iDestruct (auth_nat_max_auth_agree with "Hback_auth₁ Hback_auth₂") as %->.
+    iCombine "Hback_auth₁ Hback_auth₂" as "Hback_auth".
+    iMod (auth_nat_max_update with "Hback_auth") as "(Hback_auth₁ & Hback_auth₂)"; first done.
+    iSteps.
   Qed.
-  #[local] Lemma back_lb_get γ back :
-    producer_ctl₂ γ back ⊢
+  #[local] Lemma back_lb_get γ stable back :
+    producer₂ γ stable back ⊢
     back_lb γ back.
   Proof.
-    apply auth_nat_max_lb_get.
+    iIntros "(:producer₂)".
+    iApply (auth_nat_max_lb_get with "Hback_auth₂").
   Qed.
-  #[local] Lemma back_lb_valid γ back1 back2 :
-    producer_ctl₂ γ back1 -∗
+  #[local] Lemma back_lb_valid γ stable back1 back2 :
+    producer₂ γ stable back1 -∗
     back_lb γ back2 -∗
     ⌜back2 ≤ back1⌝.
   Proof.
-    apply auth_nat_max_lb_valid.
+    iIntros "(:producer₂) Hback_lb".
+    iApply (auth_nat_max_lb_valid with "Hback_auth₂ Hback_lb").
   Qed.
 
-  #[local] Lemma producer_region_alloc :
+  #[local] Lemma consumer_alloc :
     ⊢ |==>
-      ∃ γ_producer_region,
-      producer_region' γ_producer_region.
+      ∃ γ_consumer γ_front,
+      consumer₁' γ_consumer γ_front Stable 0 ∗
+      consumer₂' γ_consumer γ_front Stable 0.
   Proof.
-    apply excl_alloc.
-  Qed.
-  #[local] Lemma producer_region_exclusive γ :
-    producer_region γ -∗
-    producer_region γ -∗
-    False.
-  Proof.
-    apply excl_exclusive.
-  Qed.
-
-  #[local] Lemma consumer_ctl_alloc :
-    ⊢ |==>
-      ∃ γ_consumer_ctl,
-      consumer_ctl₁' γ_consumer_ctl 0 ∗
-      consumer_ctl₂' γ_consumer_ctl 0.
-  Proof.
-    iMod auth_nat_max_alloc as "(%γ_consumer_ctl & Hconsumer_ctl₁ & Hconsumer_ctl₂)".
+    iMod twins_alloc' as "(%γ_consumer & Hconsumer₁ & Hconsumer₂)".
+    iMod auth_nat_max_alloc as "(%γ_front & Hfront_auth₁ & Hfront_auth₂)".
     iSteps.
   Qed.
-  #[local] Lemma consumer_ctl_agree γ front1 front2 :
-    consumer_ctl₁ γ front1 -∗
-    consumer_ctl₂ γ front2 -∗
-    ⌜front1 = front2⌝.
+  #[local] Lemma consumer_agree γ stable1 front1 stable2 front2 :
+    consumer₁ γ stable1 front1 -∗
+    consumer₂ γ stable2 front2 -∗
+      ⌜stable1 = stable2⌝ ∗
+      ⌜front1 = front2⌝.
   Proof.
-    apply auth_nat_max_auth_agree.
+    iIntros "(:consumer₁) (:consumer₂)".
+    iDestruct (twins_agree_L with "Hconsumer₁ Hconsumer₂") as %<-.
+    iDestruct (auth_nat_max_auth_agree with "Hfront_auth₁ Hfront_auth₂") as %<-.
+    iSteps.
   Qed.
-  #[local] Lemma consumer_ctl_update {γ front1 front2} front :
+  #[local] Lemma consumer_update_front {γ stable1 front1 stable2 front2} front :
     front1 ≤ front →
-    consumer_ctl₁ γ front1 -∗
-    consumer_ctl₂ γ front2 ==∗
-      consumer_ctl₁ γ front ∗
-      consumer_ctl₂ γ front.
+    consumer₁ γ stable1 front1 -∗
+    consumer₂ γ stable2 front2 ==∗
+      consumer₁ γ stable1 front ∗
+      consumer₂ γ stable2 front.
   Proof.
-    iIntros "%Hle Hconsumer_ctl₁ Hconsumer_ctl₂".
-    iDestruct (auth_nat_max_auth_agree with "Hconsumer_ctl₁ Hconsumer_ctl₂") as %->.
-    iCombine "Hconsumer_ctl₁ Hconsumer_ctl₂" as "Hconsumer_ctl".
-    iMod (auth_nat_max_update with "Hconsumer_ctl") as "($ & $)"; done.
+    iIntros "% (:consumer₁) (:consumer₂)".
+    iDestruct (auth_nat_max_auth_agree with "Hfront_auth₁ Hfront_auth₂") as %->.
+    iCombine "Hfront_auth₁ Hfront_auth₂" as "Hfront_auth".
+    iMod (auth_nat_max_update with "Hfront_auth") as "(Hauth_auth₁ & Hfront_auth₂)"; first done.
+    iSteps.
   Qed.
-  #[local] Lemma front_lb_get γ front :
-    consumer_ctl₂ γ front ⊢
+  #[local] Lemma consumer_update_stability {γ stable1 front1 stable2 front2} stable :
+    consumer₁ γ stable1 front1 -∗
+    consumer₂ γ stable2 front2 ==∗
+      consumer₁ γ stable front1 ∗
+      consumer₂ γ stable front2.
+  Proof.
+    iIntros "(:consumer₁) (:consumer₂)".
+    iMod (twins_update' with "Hconsumer₁ Hconsumer₂") as "(Hconsumer₁ & Hconsumer₂)".
+    iSteps.
+  Qed.
+  #[local] Lemma front_lb_get γ stable front :
+    consumer₂ γ stable front ⊢
     front_lb γ front.
   Proof.
-    apply auth_nat_max_lb_get.
+    iIntros "(:consumer₂)".
+    iApply (auth_nat_max_lb_get with "Hfront_auth₂").
   Qed.
-  #[local] Lemma front_lb_valid γ front1 front2 :
-    consumer_ctl₂ γ front1 -∗
+  #[local] Lemma front_lb_valid γ stable front1 front2 :
+    consumer₂ γ stable front1 -∗
     front_lb γ front2 -∗
     ⌜front2 ≤ front1⌝.
   Proof.
-    iIntros "Hconsumer_ctl₁ Hfront_lb".
-    iApply (auth_nat_max_lb_valid with "Hconsumer_ctl₁ Hfront_lb").
+    iIntros "(:consumer₂) Hfront_lb".
+    iApply (auth_nat_max_lb_valid with "Hfront_auth₂ Hfront_lb").
   Qed.
 
-  #[local] Lemma consumer_region_alloc :
-    ⊢ |==>
-      ∃ γ_consumer_region,
-      consumer_region' γ_consumer_region.
-  Proof.
-    apply excl_alloc.
-  Qed.
-  #[local] Lemma consumer_region_exclusive γ :
-    consumer_region γ -∗
-    consumer_region γ -∗
-    False.
-  Proof.
-    apply excl_exclusive.
-  Qed.
-
-  Opaque producer_ctl₁'.
+  Opaque producer₁'.
+  Opaque producer₂'.
+  Opaque consumer₁'.
+  Opaque consumer₂'.
 
   Lemma spsc_bqueue_producer_exclusive t ws :
     spsc_bqueue_producer t ws -∗
@@ -475,7 +512,7 @@ Section spsc_bqueue_G.
   Proof.
     iIntros "(:producer =) (:model)". injection Heq as <-.
     iDestruct (meta_agree with "Hmeta Hmeta_") as %<-. iClear "Hmeta_".
-    iApply (model_valid with "Hproducer_ctl₁ Hmodel₁").
+    iApply (model_valid with "Hproducer₁ Hmodel₁").
   Qed.
 
   Lemma spsc_bqueue_consumer_exclusive t :
@@ -515,31 +552,29 @@ Section spsc_bqueue_G.
     wp_block l as "Hmeta" "(Hl_data & Hl_front & Hl_front_cache & Hl_back & Hl_back_cache & _)".
     iMod (pointsto_persist with "Hl_data") as "#Hl_data".
 
-    iMod model_producer_ctl_alloc as "(%γ_model & %γ_producer_ctl & Hmodel₁ & Hmodel₂ & Hproducer_ctl₁ & Hproducer_ctl₂)".
+    iMod model_producer_alloc as "(%γ_model & %γ_producer & %γ_back & Hmodel₁ & Hmodel₂ & Hproducer₁ & Hproducer₂)".
     iMod history_alloc as "(%γ_history & Hhistory_auth)".
-    iMod producer_region_alloc as "(%γ_producer_region & Hproducer_region)".
-    iMod consumer_ctl_alloc as "(%γ_consumer_ctl & Hconsumer_ctl₁ & Hconsumer_ctl₂)".
-    iMod consumer_region_alloc as "(%γ_consumer_region & Hconsumer_region)".
+    iMod consumer_alloc as "(%γ_consumer & %γ_front & Hconsumer₁ & Hconsumer₂)".
 
     pose γ := {|
       metadata_capacity := ₊cap ;
       metadata_data := data ;
       metadata_model := γ_model ;
       metadata_history := γ_history ;
-      metadata_producer_ctl := γ_producer_ctl ;
-      metadata_producer_region := γ_producer_region ;
-      metadata_consumer_ctl := γ_consumer_ctl ;
-      metadata_consumer_region := γ_consumer_region ;
+      metadata_producer := γ_producer ;
+      metadata_back := γ_back ;
+      metadata_consumer := γ_consumer ;
+      metadata_front := γ_front ;
     |}.
     iMod (meta_set _ _ γ with "Hmeta") as "#Hmeta"; first done.
 
-    iDestruct (back_lb_get γ with "Hproducer_ctl₂") as "#Hback_lb".
-    iDestruct (front_lb_get γ with "Hconsumer_ctl₂") as "#Hfront_lb".
+    iDestruct (back_lb_get γ with "Hproducer₂") as "#Hback_lb".
+    iDestruct (front_lb_get γ with "Hconsumer₂") as "#Hfront_lb".
 
     iApply "HΦ".
-    iSplitL "Hdata_model Hl_front Hl_back Hmodel₂ Hhistory_auth Hproducer_ctl₂ Hconsumer_ctl₂"; last iSteps.
+    iSplitL "Hdata_model Hl_front Hl_back Hmodel₂ Hhistory_auth Hproducer₂ Hconsumer₂"; last iSteps.
     iExists l, γ. iStep 5.
-    iApply inv_alloc. iExists 0, 0, [], []. iStep 11.
+    iApply inv_alloc. iExists Stable, 0, Stable, 0, [], []. iStep 11.
     Z_to_nat cap. rewrite Nat2Z.id. destruct cap as [| cap]; first iSteps.
     iDestruct (array_model_to_cslice with "Hdata_model") as "Hdata_cslice".
     rewrite length_replicate -(take_drop 1 (replicate _ _)).
@@ -548,43 +583,43 @@ Section spsc_bqueue_G.
     rewrite Nat.sub_0_r. iSteps.
   Qed.
 
-  #[local] Lemma spsc_bqueue_front_spec l γ ι front :
+  #[local] Lemma spsc_bqueue_front_spec l γ ι stable front :
     {{{
       inv ι (inv_inner l γ) ∗
-      consumer_ctl₁ γ front
+      consumer₁ γ stable front
     }}}
       (#l).{front}
     {{{
       RET #front;
-      consumer_ctl₁ γ front
+      consumer₁ γ stable front
     }}}.
   Proof.
-    iIntros "%Φ (#Hinv & Hconsumer_ctl₁) HΦ".
+    iIntros "%Φ (#Hinv & Hconsumer₁) HΦ".
 
     iInv "Hinv" as "(:inv_inner =')".
     wp_load.
-    iDestruct (consumer_ctl_agree with "Hconsumer_ctl₁ Hconsumer_ctl₂") as %<-.
-    iSplitR "Hconsumer_ctl₁ HΦ". { iFrameSteps. }
+    iDestruct (consumer_agree with "Hconsumer₁ Hconsumer₂") as %(<- & <-).
+    iSplitR "Hconsumer₁ HΦ". { iFrameSteps. }
     iSteps.
   Qed.
 
-  #[local] Lemma spsc_bqueue_back_spec l γ ι back ws :
+  #[local] Lemma spsc_bqueue_back_spec l γ ι stable back ws :
     {{{
       inv ι (inv_inner l γ) ∗
-      producer_ctl₁ γ back ws
+      producer₁ γ stable back ws
     }}}
       (#l).{back}
     {{{
       RET #back;
-      producer_ctl₁ γ back ws
+      producer₁ γ stable back ws
     }}}.
   Proof.
-    iIntros "%Φ (#Hinv & Hproducer_ctl₁) HΦ".
+    iIntros "%Φ (#Hinv & Hproducer₁) HΦ".
 
     iInv "Hinv" as "(:inv_inner =')".
     wp_load.
-    iDestruct (producer_ctl_agree with "Hproducer_ctl₁ Hproducer_ctl₂") as %<-.
-    iSplitR "Hproducer_ctl₁ HΦ". { iFrameSteps. }
+    iDestruct (producer_agree with "Hproducer₁ Hproducer₂") as %(<- & <-).
+    iSplitR "Hproducer₁ HΦ". { iFrameSteps. }
     iSteps.
   Qed.
 
@@ -607,20 +642,20 @@ Section spsc_bqueue_G.
 
     wp_rec.
 
-    wp_apply (spsc_bqueue_back_spec with "[$Hinv $Hproducer_ctl₁]") as "Hproducer_ctl₁".
+    wp_apply (spsc_bqueue_back_spec with "[$Hinv $Hproducer₁]") as "Hproducer₁".
     wp_pures.
 
     wp_bind (_.{front})%E.
     iInv "Hinv" as "(:inv_inner =2)".
     wp_load.
-    iDestruct (producer_ctl_agree with "Hproducer_ctl₁ Hproducer_ctl₂") as %<-.
+    iDestruct (producer_agree with "Hproducer₁ Hproducer₂") as %(<- & <-).
 
     iMod "HΦ" as "(%vs & (:model) & _ & HΦ)". injection Heq as <-.
     iDestruct (meta_agree with "Hmeta Hmeta_") as %<-. iClear "Hmeta_".
     iDestruct (model_agree with "Hmodel₁ Hmodel₂") as %<-.
     iMod ("HΦ" with "[$Hmodel₁]") as "HΦ"; first iSteps.
 
-    iSplitR "Hl_front_cache Hproducer_ctl₁ Hproducer_region HΦ". { iFrameSteps. }
+    iSplitR "Hl_front_cache Hproducer₁ HΦ". { iFrameSteps. }
     assert (⁺back - ⁺front2 = length vs)%Z as Hlen by lia.
     iModIntro. clear- Hlen.
 
@@ -648,18 +683,18 @@ Section spsc_bqueue_G.
     wp_bind (_.{back})%E.
     iInv "Hinv" as "(:inv_inner =1)".
     wp_load.
-    iDestruct (consumer_ctl_agree with "Hconsumer_ctl₁ Hconsumer_ctl₂") as %<-.
+    iDestruct (consumer_agree with "Hconsumer₁ Hconsumer₂") as %(<- & <-).
 
     iMod "HΦ" as "(%vs & (:model) & _ & HΦ)". injection Heq as <-.
     iDestruct (meta_agree with "Hmeta Hmeta_") as %<-. iClear "Hmeta_".
     iDestruct (model_agree with "Hmodel₁ Hmodel₂") as %<-.
     iMod ("HΦ" with "[$Hmodel₁]") as "HΦ"; first iSteps.
 
-    iSplitR "Hl_back_cache Hconsumer_ctl₁ Hconsumer_region HΦ". { iFrameSteps. }
+    iSplitR "Hl_back_cache Hconsumer₁ HΦ". { iFrameSteps. }
     assert (⁺back1 - ⁺front = length vs)%Z as Hlen by lia.
     iModIntro. clear- Hlen.
 
-    wp_smart_apply (spsc_bqueue_front_spec with "[$Hinv $Hconsumer_ctl₁]") as "Hconsumer_ctl₁".
+    wp_smart_apply (spsc_bqueue_front_spec with "[$Hinv $Hconsumer₁]") as "Hconsumer₁".
     iSteps. rewrite Hlen. iSteps.
   Qed.
 
@@ -725,13 +760,13 @@ Section spsc_bqueue_G.
     COMM
       Ψ vs
     }>.
-  #[local] Lemma spsc_bqueue_push_0_spec l ι γ front_cache back ws v Ψ :
+  #[local] Lemma spsc_bqueue_push_0_spec l ι γ front_cache stable back ws v Ψ :
     {{{
       meta l nroot γ ∗
       array_inv γ.(metadata_data) γ.(metadata_capacity) ∗
       inv ι (inv_inner l γ) ∗
       l.[front_cache] ↦ #front_cache ∗
-      producer_ctl₁ γ back ws ∗
+      producer₁ γ stable back ws ∗
       front_lb γ front_cache ∗
       au_push l γ ι v Ψ
     }}}
@@ -740,7 +775,7 @@ Section spsc_bqueue_G.
       RET #b;
       ⌜b = bool_decide (back < front_cache + γ.(metadata_capacity))⌝ ∗
       l.[front_cache] ↦ #front_cache ∗
-      producer_ctl₁ γ back ws ∗
+      producer₁ γ stable back ws ∗
       front_lb γ front_cache ∗
       if b then
         au_push l γ ι v Ψ
@@ -750,7 +785,7 @@ Section spsc_bqueue_G.
         Ψ vs
     }}}.
   Proof.
-    iIntros "%Φ (#Hmeta & #Hdata_inv & #Hinv & Hl_front_cache & Hproducer_ctl₁ & #Hfront_lb & HΨ) HΦ".
+    iIntros "%Φ (#Hmeta & #Hdata_inv & #Hinv & Hl_front_cache & Hproducer₁ & #Hfront_lb & HΨ) HΦ".
 
     wp_rec.
     wp_smart_apply (array_size_spec_inv with "Hdata_inv") as "_".
@@ -763,11 +798,11 @@ Section spsc_bqueue_G.
     - wp_bind (_.{front})%E.
       iInv "Hinv" as "(:inv_inner =1)".
       wp_load.
-      iDestruct (producer_ctl_agree with "Hproducer_ctl₁ Hproducer_ctl₂") as %<-.
-      iClear "Hfront_lb". iDestruct (front_lb_get with "Hconsumer_ctl₂") as "#Hfront_lb".
+      iDestruct (producer_agree with "Hproducer₁ Hproducer₂") as %(<- & <-).
+      iClear "Hfront_lb". iDestruct (front_lb_get with "Hconsumer₂") as "#Hfront_lb".
       destruct (decide (back < front1 + γ.(metadata_capacity))) as [Hbranch2 | Hbranch2].
 
-      + iSplitR "Hl_front_cache Hproducer_ctl₁ HΨ HΦ". { iFrameSteps. }
+      + iSplitR "Hl_front_cache Hproducer₁ HΨ HΦ". { iFrameSteps. }
         iModIntro. clear- Hbranch2.
 
         wp_store. wp_pures.
@@ -782,7 +817,7 @@ Section spsc_bqueue_G.
         rewrite decide_True; [lia.. |].
         iMod ("HΨ" with "[Hmodel₁]") as "HΨ"; first iSteps.
 
-        iSplitR "Hl_front_cache Hproducer_ctl₁ HΨ HΦ". { iFrameSteps. }
+        iSplitR "Hl_front_cache Hproducer₁ HΨ HΦ". { iFrameSteps. }
         iModIntro. clear- Hbranch2 Hvs1_len.
 
         wp_store. wp_pures.
@@ -807,58 +842,56 @@ Section spsc_bqueue_G.
     iDestruct (meta_agree with "Hmeta Hmeta_") as %<-. iClear "Hmeta_".
 
     wp_rec. wp_load.
-    wp_smart_apply (spsc_bqueue_back_spec with "[$Hinv $Hproducer_ctl₁]") as "Hproducer_ctl₁".
-    iDestruct "Hfront_lb" as "-#Hfront_lb". wp_smart_apply (spsc_bqueue_push_0_spec with "[$]") as (? front_cache') "(-> & Hl_front_cache & Hproducer_ctl₁ & #Hfront_lb & HΦ)".
+    wp_smart_apply (spsc_bqueue_back_spec with "[$Hinv $Hproducer₁]") as "Hproducer₁".
+    iDestruct "Hfront_lb" as "-#Hfront_lb". wp_smart_apply (spsc_bqueue_push_0_spec with "[$]") as (? front_cache') "(-> & Hl_front_cache & Hproducer₁ & #Hfront_lb & HΦ)".
     case_bool_decide as Hbranch.
 
     - iApply fupd_wp.
       iInv "Hinv" as "(:inv_inner =2)".
-      iDestruct (producer_ctl_agree with "Hproducer_ctl₁ Hproducer_ctl₂") as %<-.
-      iDestruct "Hback" as "[Hback_ | Hproducer_region_]"; last first.
-      { iDestruct (producer_region_exclusive with "Hproducer_region Hproducer_region_") as %[]. }
-      iDestruct (front_lb_valid with "Hconsumer_ctl₂ Hfront_lb") as %Hfront2.
+      iDestruct (producer_agree with "Hproducer₁ Hproducer₂") as %(<- & <-).
+      iDestruct (front_lb_valid with "Hconsumer₂ Hfront_lb") as %Hfront2.
       rewrite decide_False; first lia.
-      iSplitR "Hl_front_cache Hproducer_ctl₁ Hback_ HΦ". { iFrameSteps. }
+      iMod (producer_update_stability Unstable with "Hproducer₁ Hproducer₂") as "(Hproducer₁ & Hproducer₂)".
+      iSplitR "Hl_front_cache Hproducer₁ Hback HΦ". { iFrameSteps. }
       iModIntro. clear- Hbranch. iModIntro.
 
-      wp_smart_apply (array_unsafe_cset_spec with "Hback_") as "Hback_"; first done.
+      wp_smart_apply (array_unsafe_cset_spec with "Hback") as "Hback_"; first done.
       wp_pures.
 
       wp_bind (_ <-{back} _)%E.
       iInv "Hinv" as "(:inv_inner =3)".
       wp_store.
-      iDestruct (producer_ctl_agree with "Hproducer_ctl₁ Hproducer_ctl₂") as %<-.
-      iDestruct (front_lb_valid with "Hconsumer_ctl₂ Hfront_lb") as %Hfront3_ge.
-      iDestruct "Hback" as "[Hback | Hproducer_region]".
-      { rewrite decide_False; first lia.
-        iDestruct (array_cslice_exclusive with "Hback Hback_") as %[]; [simpl; lia | done].
-      }
-      iMod (producer_ctl_update (S back) with "Hproducer_ctl₁ Hproducer_ctl₂") as "(Hproducer_ctl₁ & Hproducer_ctl₂)"; first lia.
+      iDestruct (producer_agree with "Hproducer₁ Hproducer₂") as %(<- & <-).
+      iDestruct (front_lb_valid with "Hconsumer₂ Hfront_lb") as %Hfront3_ge.
+      iMod (producer_update_stability Stable with "Hproducer₁ Hproducer₂") as "(Hproducer₁ & Hproducer₂)".
+      iMod (producer_update_back (S back) with "Hproducer₁ Hproducer₂") as "(Hproducer₁ & Hproducer₂)"; first lia.
       iMod (history_update v with "Hhistory_auth") as "Hhistory_auth".
 
       iMod "HΦ" as "(%vs & (:model) & _ & HΦ)". injection Heq as <-.
       iDestruct (meta_agree with "Hmeta Hmeta_") as %<-. iClear "Hmeta_".
       iDestruct (model_agree with "Hmodel₁ Hmodel₂") as %->.
-      iMod (model_push v with "Hproducer_ctl₁ Hmodel₁ Hmodel₂") as "(Hproducer_ctl₁ & Hmodel₁ & Hmodel₂)".
+      iMod (model_push v with "Hproducer₁ Hmodel₁ Hmodel₂") as "(Hproducer₁ & Hmodel₁ & Hmodel₂)".
       rewrite !decide_False; [lia.. |]. rewrite bool_decide_eq_false_2; first lia.
       iMod ("HΦ" with "[Hmodel₁]") as "HΦ"; first iSteps.
 
-      iSplitR "Hl_front_cache Hproducer_ctl₁ Hproducer_region HΦ".
-      { do 2 iModIntro. iExists front3, (S back), (vs3 ++ [v]), (hist3 ++ [v]). iFrame.
+      iSplitR "Hl_front_cache Hproducer₁ HΦ".
+      { do 2 iModIntro. iExists _, front3, _, (S back), (vs3 ++ [v]), (hist3 ++ [v]). iFrame.
         rewrite !length_app. iStep 3.
         iSplit. { rewrite Hvs3 drop_app_le //; first lia. }
-        iSplitL "Hl_back"; first iSteps.
+        iStep.
         rewrite assoc. iSplitL "Hfront Hvs Hback_".
-        - destruct vs3 as [| v' vs3].
-          + assert (front3 = back) as -> by naive_solver lia. iSteps.
-          + iFrame. rewrite /= !drop_0 fmap_app.
+        - destruct vs3 as [| v' vs3]; iFrame.
+          + assert (front3 = back) as -> by naive_solver lia.
+            destruct cstable3; iSteps.
+          + rewrite /= !drop_0 fmap_app.
             iApply (array_cslice_app_1 with "Hvs Hback_").
             rewrite length_fmap. naive_solver lia.
         - case_decide.
-          + assert (γ.(metadata_capacity) - (S back - front3) - 1 = 0) as -> by lia. iSteps.
-          + iDestruct (array_cslice_app_2 [§None%V] (replicate (γ.(metadata_capacity) - (S back - front3) - 1) §None%V) with "Hextra") as "(Hback & Hextra)".
+          + assert (γ.(metadata_capacity) - (S back - front3) - 1 = 0) as -> by lia.
+            iSteps.
+          + iDestruct (array_cslice_app_2 [§None%V] (replicate (γ.(metadata_capacity) - (S back - front3) - 1) §None%V) with "Hextra") as "($ & Hextra)".
             { rewrite /= -replicate_S. f_equal. lia. }
-            rewrite Nat.add_1_r. iSteps.
+            rewrite Nat.add_1_r //.
       }
       iSteps.
 
@@ -877,12 +910,12 @@ Section spsc_bqueue_G.
       spsc_bqueue_consumer #l -∗
       Ψ (head vs : val)
     }>.
-  #[local] Lemma spsc_bqueue_pop_0_spec l ι γ front back_cache Ψ :
+  #[local] Lemma spsc_bqueue_pop_0_spec l ι γ back_cache stable front Ψ :
     {{{
       meta l nroot γ ∗
       inv ι (inv_inner l γ) ∗
       l.[back_cache] ↦ #back_cache ∗
-      consumer_ctl₁ γ front ∗
+      consumer₁ γ stable front ∗
       back_lb γ back_cache ∗
       au_pop l ι Ψ
     }}}
@@ -891,7 +924,7 @@ Section spsc_bqueue_G.
       RET #b;
       ⌜b = bool_decide (front < back_cache)⌝ ∗
       l.[back_cache] ↦ #back_cache ∗
-      consumer_ctl₁ γ front ∗
+      consumer₁ γ stable front ∗
       back_lb γ back_cache ∗
       if b then
         au_pop l ι Ψ
@@ -900,7 +933,7 @@ Section spsc_bqueue_G.
         Ψ None
     }}}.
   Proof.
-    iIntros "%Φ (#Hmeta & #Hinv & Hl_back_cache & Hconsumer_ctl₁ & #Hback_lb & HΨ) HΦ".
+    iIntros "%Φ (#Hmeta & #Hinv & Hl_back_cache & Hconsumer₁ & #Hback_lb & HΨ) HΦ".
 
     wp_rec.
     wp_load. wp_pures.
@@ -912,11 +945,11 @@ Section spsc_bqueue_G.
     - wp_bind (_.{back})%E.
       iInv "Hinv" as "(:inv_inner =1)".
       wp_load.
-      iDestruct (consumer_ctl_agree with "Hconsumer_ctl₁ Hconsumer_ctl₂") as %<-.
-      iClear "Hback_lb". iDestruct (back_lb_get with "Hproducer_ctl₂") as "#Hback_lb".
+      iDestruct (consumer_agree with "Hconsumer₁ Hconsumer₂") as %(<- & <-).
+      iClear "Hback_lb". iDestruct (back_lb_get with "Hproducer₂") as "#Hback_lb".
       destruct (decide (front < back1)) as [Hbranch2 | Hbranch2].
 
-      + iSplitR "Hl_back_cache Hconsumer_ctl₁ HΨ HΦ". { iFrameSteps. }
+      + iSplitR "Hl_back_cache Hconsumer₁ HΨ HΦ". { iFrameSteps. }
         iModIntro. clear- Hbranch2.
 
         wp_store. wp_pures.
@@ -931,7 +964,7 @@ Section spsc_bqueue_G.
         assert (length vs1 = 0) as ->%nil_length_inv by lia.
         iMod ("HΨ" with "[Hmodel₁]") as "HΨ"; first iSteps.
 
-        iSplitR "Hl_back_cache Hconsumer_ctl₁ HΨ HΦ". { iFrameSteps. }
+        iSplitR "Hl_back_cache Hconsumer₁ HΨ HΦ". { iFrameSteps. }
         iModIntro. clear- Hbranch2.
 
         wp_store. wp_pures.
@@ -956,35 +989,34 @@ Section spsc_bqueue_G.
     iDestruct (meta_agree with "Hmeta Hmeta_") as %<-. iClear "Hmeta_".
 
     wp_rec.
-    wp_smart_apply (spsc_bqueue_front_spec with "[$Hinv $Hconsumer_ctl₁]") as "Hconsumer_ctl₁".
-    iDestruct "Hback_lb" as "-#Hback_lb". wp_smart_apply (spsc_bqueue_pop_0_spec with "[$]") as (? back_cache') "(-> & Hl_back_cache & Hconsumer_ctl₁ & #Hback_lb & HΦ)".
+    wp_smart_apply (spsc_bqueue_front_spec with "[$Hinv $Hconsumer₁]") as "Hconsumer₁".
+    iDestruct "Hback_lb" as "-#Hback_lb". wp_smart_apply (spsc_bqueue_pop_0_spec with "[$]") as (? back_cache') "(-> & Hl_back_cache & Hconsumer₁ & #Hback_lb & HΦ)".
     case_bool_decide as Hbranch; last iSteps.
 
     iApply fupd_wp.
     iInv "Hinv" as "(:inv_inner =2)".
-    iDestruct (consumer_ctl_agree with "Hconsumer_ctl₁ Hconsumer_ctl₂") as %<-.
-    iDestruct (back_lb_valid with "Hproducer_ctl₂ Hback_lb") as %Hback2_ge.
+    iDestruct (consumer_agree with "Hconsumer₁ Hconsumer₂") as %(<- & <-).
+    iDestruct (back_lb_valid with "Hproducer₂ Hback_lb") as %Hback2_ge.
     destruct vs2 as [| v vs2]; first naive_solver lia.
-    iDestruct "Hfront" as "[Hfront_ | Hconsumer_region_]"; last first.
-    { iDestruct (consumer_region_exclusive with "Hconsumer_region Hconsumer_region_") as %[]. }
     iDestruct (history_at_get front v with "Hhistory_auth") as "#Hhistory_at".
     { rewrite -(take_drop front hist2) -Hvs2 lookup_app_r length_take; first lia.
       rewrite Nat.min_l; first lia.
       rewrite Nat.sub_diag //.
     }
-    iSplitR "Hl_back_cache Hconsumer_ctl₁ Hfront_ HΦ". { iFrameSteps. }
+    iMod (consumer_update_stability Unstable with "Hconsumer₁ Hconsumer₂") as "(Hconsumer₁ & Hconsumer₂)".
+    iSplitR "Hl_back_cache Hconsumer₁ Hfront HΦ". { iFrameSteps. }
     iModIntro. clear- Hbranch. iModIntro.
 
     wp_load.
-    wp_smart_apply (array_unsafe_cget_spec with "Hfront_") as "Hfront_"; first done.
-    wp_smart_apply (array_unsafe_cset_spec with "Hfront_") as "Hfront_"; first done.
+    wp_smart_apply (array_unsafe_cget_spec with "Hfront") as "Hfront"; first done.
+    wp_smart_apply (array_unsafe_cset_spec with "Hfront") as "Hfront_"; first done.
     wp_pures.
 
     wp_bind (_ <-{front} _)%E.
     iInv "Hinv" as "(:inv_inner =3)".
     wp_store.
-    iDestruct (consumer_ctl_agree with "Hconsumer_ctl₁ Hconsumer_ctl₂") as %<-.
-    iDestruct (back_lb_valid with "Hproducer_ctl₂ Hback_lb") as %Hback2.
+    iDestruct (consumer_agree with "Hconsumer₁ Hconsumer₂") as %(<- & <-).
+    iDestruct (back_lb_valid with "Hproducer₂ Hback_lb") as %Hback2.
     destruct vs3 as [| _v vs3]; first naive_solver lia.
     iDestruct (history_agree with "Hhistory_auth Hhistory_at") as %Hhist3_lookup.
     assert (_v = v) as ->.
@@ -994,9 +1026,8 @@ Section spsc_bqueue_G.
       rewrite Nat.sub_diag. naive_solver.
     }
     rewrite /= drop_0.
-    iDestruct "Hfront" as "[Hfront | Hconsumer_region]".
-    { iDestruct (array_cslice_exclusive with "Hfront Hfront_") as %[]; [simpl; lia | done]. }
-    iMod (consumer_ctl_update (S front) with "Hconsumer_ctl₁ Hconsumer_ctl₂") as "(Hconsumer_ctl₁ & Hconsumer_ctl₂)"; first lia.
+    iMod (consumer_update_stability Stable with "Hconsumer₁ Hconsumer₂") as "(Hconsumer₁ & Hconsumer₂)".
+    iMod (consumer_update_front (S front) with "Hconsumer₁ Hconsumer₂") as "(Hconsumer₁ & Hconsumer₂)"; first lia.
 
     iMod "HΦ" as "(%vs & (:model) & _ & HΦ)". injection Heq as <-.
     iDestruct (meta_agree with "Hmeta Hmeta_") as %<-. iClear "Hmeta_".
@@ -1004,22 +1035,23 @@ Section spsc_bqueue_G.
     iMod (model_pop with "Hmodel₁ Hmodel₂") as "(Hmodel₁ & Hmodel₂)".
     iMod ("HΦ" with "[Hmodel₁]") as "HΦ"; first iSteps.
 
-    iSplitR "Hl_back_cache Hconsumer_ctl₁ Hconsumer_region HΦ".
-    { do 2 iModIntro. iExists (S front), back3, vs3, hist3. iFrame. simpl in *.
+    iSplitR "Hl_back_cache Hconsumer₁ HΦ".
+    { do 2 iModIntro. iExists _, (S front), _, back3, vs3, hist3. iFrame. simpl in *.
       iStep 3.
       iSplit. { erewrite drop_S in Hvs3 => //. naive_solver. }
       iStep.
       rewrite assoc. iSplitL "Hvs".
       - rewrite -{1}(take_drop 1 vs3) fmap_app -array_cslice_app length_fmap length_take.
-        destruct vs3; last rewrite Nat.add_1_r; iSteps.
-      - iDestruct (array_cslice_shift with "Hfront_") as "Hfront".
+        destruct vs3.
+        2: rewrite Nat.add_1_r.
+        all: destruct pstable3; iSteps.
+      - iDestruct (array_cslice_shift with "Hfront_") as "Hfront_".
         case_decide as Hcase.
         + rewrite -Hcase decide_False; first lia.
           assert (γ.(metadata_capacity) - (back3 - S front) - 1 = 0) as -> by lia.
-          iSteps.
-        + rewrite decide_False; first lia.
-          iFrame.
-          iDestruct (array_cslice_app_1 with "Hextra Hfront") as "Hextra".
+          destruct pstable3; iSteps.
+        + rewrite decide_False; first lia. iFrame.
+          iDestruct (array_cslice_app_1 with "Hextra Hfront_") as "Hextra".
           { rewrite length_replicate. lia. }
           rewrite -replicate_S_end.
           assert (S (γ.(metadata_capacity) - (back3 - front) - 1) = γ.(metadata_capacity) - (back3 - S front) - 1) as -> by lia.
